Attempts to get gctr_partial_opaque_ignores_postfix triggering correctly

vale/code/crypto/aes/GCTR.fsti
@@ -60,7 +60,27 @@ let gctr_partial_opaque_ignores_postfix (alg:algorithm) (bound:nat) (plain plain
   (ensures gctr_partial_opaque alg bound plain cipher key icb == gctr_partial_opaque alg bound plain' cipher' key icb)
   =
   reveal_opaque gctr_partial;
-  admit();
+  let helper i : Lemma (0 <= i /\ i < bound ==> 
+                          (index cipher  i == quad32_xor (index plain  i) (aes_encrypt_BE alg key (inc32 icb i))) ==
+                          (index cipher' i == quad32_xor (index plain' i) (aes_encrypt_BE alg key (inc32 icb i))))
+    =
+    if 0 <= i && i < bound then (      
+      assert (index plain i == index (slice plain 0 bound) i);  // OBSERVE
+      assert (index cipher i == index (slice cipher 0 bound) i);  // OBSERVE
+      assert (index cipher i == index cipher' i);
+      assert (index plain i  == index plain'  i);
+      ()
+    ) else ();
+    ()
+  in
+  FStar.Classical.forall_intro helper;
+  assert (forall i . 0 <= i /\ i < bound ==> index plain i == index (slice plain 0 bound) i);
+  assert (forall i . 0 <= i /\ i < bound ==> index plain' i == index (slice plain' 0 bound) i);
+  assert (forall i . 0 <= i /\ i < bound ==> index cipher i == index (slice cipher 0 bound) i);
+  assert (forall i . 0 <= i /\ i < bound ==> index cipher' i == index (slice cipher' 0 bound) i);
+  assert (gctr_partial_opaque alg bound plain cipher key icb == gctr_partial alg bound plain cipher key icb);
+  assert (gctr_partial_opaque alg bound plain' cipher' key icb == gctr_partial alg bound plain' cipher' key icb);  
+  admit(); 
   ()
 
 let gctr_partial_extend6 (alg:algorithm) (bound:nat) (plain cipher:seq quad32) (key:seq nat32) (icb:quad32) : Lemma
